src/dvspec/dafny/att_spec_proofs/dvc_ind_inv.dfy
@@ -1,0 +1,142 @@
+include "../commons.dfy"
+include "../specification/dvc_spec.dfy"
+include "../specification/consensus.dfy"
+include "../specification/network.dfy"
+include "../specification/dvn.dfy"
+include "../att_spec_proofs/inv.dfy"
+include "../att_spec_proofs/assump.dfy"
+
+module DVN_Ind_Inv
+{
+    import opened Types 
+    import opened CommonFunctions
+    import opened ConsensusSpec
+    import opened NetworkSpec
+    import opened DVCNode_Spec
+    import opened DV
+    import opened Att_Inv_With_Empty_Initial_Attestation_Slashing_DB
+    import opened Att_Assumptions
+
+    lemma dvc_init_inv51(        
+        dvn: DVState,
+        hn: BLSPubkey,
+        dv_pubkey: BLSPubkey,
+        peers: set<BLSPubkey>,
+        construct_signed_attestation_signature: (set<AttestationShare>) -> Optional<BLSSignature>,
+        initial_attestation_slashing_db: set<SlashingDBAttestation>,
+        rs_pubkey: BLSPubkey
+    )
+    requires && is_honest_node(dvn, hn)
+             && var hn_state := dvn.honest_nodes_states[hn];
+             && DVCNode_Spec.Init(hn_state, dv_pubkey, peers, construct_signed_attestation_signature, 
+                    initial_attestation_slashing_db, rs_pubkey)
+    ensures && var hn_state := dvn.honest_nodes_states[hn];
+            && forall s: Slot :: inv51_body.requires(hn_state, s) ==> inv51_body(hn_state, s)
+    {}    
+
+    lemma dvc_init_inv5(        
+        dvn: DVState,
+        hn: BLSPubkey,
+        dv_pubkey: BLSPubkey,
+        peers: set<BLSPubkey>,
+        construct_signed_attestation_signature: (set<AttestationShare>) -> Optional<BLSSignature>,
+        initial_attestation_slashing_db: set<SlashingDBAttestation>,
+        rs_pubkey: BLSPubkey
+    )
+    requires && is_honest_node(dvn, hn)
+             && var hn_state := dvn.honest_nodes_states[hn];
+             && DVCNode_Spec.Init(hn_state, dv_pubkey, peers, construct_signed_attestation_signature, 
+                    initial_attestation_slashing_db, rs_pubkey)
+    ensures && var hn_state := dvn.honest_nodes_states[hn];
+            && inv5_body.requires(hn_state) ==> inv5_body(hn_state)
+    {}  
+
+    lemma {:axiom} assump_inv5_body(hn_state: DVCNodeState)
+    ensures inv5_body(hn_state)
+
+    lemma dvc_next_inv5(        
+        hn_state: DVCNodeState,
+        hn_state': DVCNodeState
+    )
+    requires && ( exists e: Types.Event, output: Outputs :: DVCNode_Spec.Next(hn_state, e, hn_state', output) ) 
+             && inv5_body(hn_state)
+    ensures inv5_body(hn_state')
+    {
+        var e: Types.Event, outputs: Outputs :| DVCNode_Spec.Next(hn_state, e, hn_state', outputs);
+
+        if e.ServeAttstationDuty? 
+        { assump_inv5_body(hn_state'); }        
+        else if e.AttConsensusDecided? 
+        { 
+            assump_inv5_body(hn_state'); 
+        }
+        else if e.ReceviedAttesttionShare?
+        { 
+            var share: AttestationShare :| f_listen_for_attestation_shares(hn_state, share).state == hn_state';
+        }
+        else if e.ImportedNewBlock?
+        { 
+            if ( exists block: BeaconBlock :: f_listen_for_new_imported_blocks.requires(hn_state, block) )
+            {
+                var block: BeaconBlock :| 
+                    && f_listen_for_new_imported_blocks.requires(hn_state, block)
+                    && f_listen_for_new_imported_blocks(hn_state, block).state == hn_state';
+                assert f_listen_for_new_imported_blocks(hn_state, block).state == hn_state';
+                // assump_inv5_body(hn_state');             
+            }
+            else
+            {}            
+        }
+        else if e.ResendAttestationShares?
+        {             
+            assert f_resend_attestation_share(hn_state).state == hn_state';
+        }        
+        else 
+        {
+            assert && e.NoEvent?
+                   && inv5_body(hn_state');
+        }
+    } 
+
+    lemma dvc_init_inv10(        
+        dvn: DVState,
+        hn: BLSPubkey,
+        dv_pubkey: BLSPubkey,
+        peers: set<BLSPubkey>,
+        construct_signed_attestation_signature: (set<AttestationShare>) -> Optional<BLSSignature>,
+        initial_attestation_slashing_db: set<SlashingDBAttestation>,
+        rs_pubkey: BLSPubkey
+    )
+    requires && is_honest_node(dvn, hn)
+             && var hn_state := dvn.honest_nodes_states[hn];
+             && DVCNode_Spec.Init(hn_state, dv_pubkey, peers, construct_signed_attestation_signature, 
+                    initial_attestation_slashing_db, rs_pubkey)
+    ensures && var hn_state := dvn.honest_nodes_states[hn];
+            && inv10_body(hn_state)
+    {}  
+
+    lemma dvc_next_inv10(        
+        hn_state: DVCNodeState,
+        hn_state': DVCNodeState
+    )
+    requires && ( exists e: Types.Event, output: Outputs :: DVCNode_Spec.Next(hn_state, e, hn_state', output) ) 
+             && inv10_body(hn_state)
+    ensures inv10_body(hn_state)
+    {} 
+
+
+/*    
+    lemma dvc_next_inv51(hn_state: DVCNodeState, hn_state': DVCNodeState)       
+    requires && ( forall s: Slot :: inv51_body.requires(hn_state, s) ==> inv51_body(hn_state, s) )
+             && ( exists e: Types.Event, output: Outputs :: DVCNode_Spec.Next(hn_state, e, hn_state', output) )            
+    ensures ( forall s: Slot :: inv51_body.requires(hn_state', s) ==> inv51_body(hn_state', s) )
+    {}
+
+    lemma dvn_next_inv52(dvn: DVState, dvn': DVState)       
+    requires exists e: DV.Event :: DV.NextEvent(dvn, e, dvn')
+    requires inv52(dvn)
+    ensures inv52(dvn')
+    {}
+ */
+    
+}
